embedding/theories/SimpleBlockchain.v
@@ -10,7 +10,7 @@ From Coq Require Import List.
 
 From MetaCoq.Template Require Import All.
 
-Import MonadNotation.
+Import MCMonadNotation.
 
 Import ListNotations.
 Import BaseTypes.
